extraction/examples/crowdfunding_extract/Crowdfunding.v
@@ -1,0 +1,192 @@
+(**  We develop a deep embedding of a crowdfunding contract and prove some of its functional correctness properties using the corresponding shallow embedding *)
+
+Require Import String ZArith Basics.
+From ConCert.Embedding Require Import Ast Notations CustomTactics
+     PCUICTranslate PCUICtoTemplate Utils MyEnv.
+
+From ConCert.Extraction Require Import Liquidity.
+From ConCert.Extraction.Examples Require Import Prelude CrowdfundingData SimpleBlockchain.
+
+Require Import List PeanoNat ssrbool.
+
+Import ListNotations.
+From MetaCoq.Template Require Import All.
+
+Import MonadNotation.
+Import BaseTypes.
+Open Scope list.
+
+Import Lia.
+
+(** Note that we define the deep embedding (abstract syntax trees) of the data structures and programs using notations. These notations are defined in  [Ast.v] and make use of the "custom entries" feature. *)
+
+(** Brackets like [[\ \]] delimit the scope of data type definitions and like [[| |]] the scope of programs *)
+
+
+(** * The crowdfunding contract *)
+
+Module CrowdfundingContract.
+
+  Import AcornBlockchain.
+
+  (** Generating string constants for variable names *)
+
+  Run TemplateProgram (mkNames ["c";"s";"e";"m";"v";"dl"; "g"; "chain";
+                                  "tx_amount"; "bal"; "sender"; "own"; "isdone" ;
+                                    "accs"; "now"; "newstate"; "newmap"; "cond" ] "").
+
+
+  (** ** AST of the [init] function *)
+  Module Init.
+    Import Notations.
+    Definition crowdfunding_init : expr :=
+      [| \own : address => \dl : time => \g : money =>
+         mkFullState (mkParams dl g own) (mkState MNil False) |].
+
+    Make Definition init :=
+      (expr_to_tc Σ' (indexify nil crowdfunding_init)).
+
+    Check init.
+ End Init.
+
+ (** ** AST of the [receive] function *)
+ Module Receive.
+
+   Import CrowdfundingData.Notations.
+     (** Constructors. [Res] is an abbreviation for [Some (st, [action]) : option (State * list ActionBody)] *)
+
+  Definition actions_ty := [! "list" "SimpleActionBody" !].
+
+  Notation "'Result'" := [!"prod"  ("list" "SimpleActionBody") {full_state_ty} !]
+                           (in custom type at level 2).
+
+  Notation "'Transfer' a b" :=
+    [| {eConstr SActionBody "Act_transfer"} {b} {a} |]
+      (in custom expr at level 0,
+          a custom expr at level 1,
+          b custom expr at level 1).
+
+  Definition eqb_addr (a1 a2 : address_coq) :=
+    match a1, a2 with
+    | ContractAddr_coq n1, ContractAddr_coq n2 => Nat.eqb n1 n2
+    | UserAddr_coq n1, UserAddr_coq n2 => Nat.eqb n1 n2
+    | _, _ => false
+    end.
+
+  Notation "a ==a b" := [| {eConst "eqb_addr"} {a} {b} |]
+                        (in custom expr at level 0).
+
+
+   (** We specialise some polymorphic constructors to avoid writing types all the time *)
+   Notation "'#Just' a" := [| $Just$Maybe  [: Result ] {a}|]
+                           (in custom expr at level 0,
+                               a custom expr at level 1).
+
+   Notation "'#Pair' a b" := [| $"pair"$"prod" [: {actions_ty}] [: {full_state_ty}] {a} {b} |]
+                           (in custom expr at level 0,
+                               a custom expr at level 1,
+                               b custom expr at level 1).
+
+   Notation "'#Nothing'" := (eApp (eConstr "option" "None") (eTy [!Result!]))
+                              (in custom expr at level 0).
+
+   Notation "'#Nil'" := [| {eConstr "list" "nil"} {eTy (tyInd SActionBody)} |]
+                      (in custom expr at level 0).
+   Notation "[ x ]" := [| {eConstr "list" "cons"} {eTy (tyInd SActionBody)} {x} #Nil |]
+                        ( in custom expr at level 0,
+                          x custom expr at level 1).
+
+
+
+   Notation "'DONE'" := (eConst "set_done")
+                          (in custom expr at level 0).
+   Notation "'UPDATE_CONTRIBS'" := (eConst "update_contribs")
+                                    (in custom expr at level 0).
+
+   Definition lookup k m := lookup_map m k.
+
+   Notation "'findm' a b" :=  [| {eConst "lookup"} {a} {b} |]
+        (in custom expr at level 0,
+            a custom expr at level 1,
+            b custom expr at level 1).
+
+   Notation SCtx := "SimpleContractCallContext".
+   Notation SChain := "SimpleChain".
+
+   Definition crowdfunding : expr :=
+     [| \sender : address => \bal : money => \tx_amount : money =>
+        \now : time => \m : msg => \s : {full_state_ty} =>
+
+         let own : address := owner s in
+         let accs : Map := contribs s in
+         case m : msg return Maybe Result of
+            | GetFunds ->
+              if (own ==a sender) && (deadline s <t now) && (goal s <= bal) then
+                #Just (#Pair [Transfer bal sender] (DONE s))
+             else #Nothing : Maybe Result
+            | Donate ->
+              if now <=t deadline s then
+                (case (findm sender accs) : Maybe money return Maybe Result of
+                  | Just v ->
+                    let newmap : Map := madd sender (v + tx_amount) accs in
+                    #Just (#Pair #Nil (UPDATE_CONTRIBS s newmap))
+                  | Nothing ->
+                    let newmap : Map := madd sender tx_amount accs in
+                    #Just (#Pair #Nil (UPDATE_CONTRIBS s newmap)))
+              else #Nothing : Maybe Result
+           | Claim ->
+             if (deadline s <t now) && (bal < goal s) && (~ done s) then
+             (case (findm sender accs) : Maybe money return Maybe Result of
+              | Just v -> let newmap : Map := madd sender 0z accs in
+                 #Just (#Pair [Transfer v sender] (UPDATE_CONTRIBS s newmap))
+              | Nothing -> #Nothing)
+             else #Nothing : Maybe Result
+    |].
+
+  Make Definition receive :=
+    (expr_to_tc Σ' (indexify nil crowdfunding)).
+
+  End Receive.
+End CrowdfundingContract.
+
+Import CrowdfundingContract.
+
+(** Packing together the data type definitions and functions *)
+Definition CFModule : LiquidityModule :=
+  {| datatypes := [msg_syn];
+     storage := [! {full_state_ty} !];
+     message := [! msg !];
+     init := Init.crowdfunding_init;
+     functions := [("update_contribs", update_contribs_syn);
+                     ("set_done", set_done_syn);
+                     ("receive", Receive.crowdfunding)
+                  ];
+     main := "receive";
+     main_extra_args:=
+       ["(Current.sender ())";
+          "(Current.balance ())";
+          "(Current.amount ())";
+          "(Current.time())"] |}.
+
+
+(** A translation table for types *)
+Definition TTty : env string :=
+  [("Coq.Numbers.BinNums.Z", "tez");
+     ("time_coq", "timestamp");
+     ("address_coq", "address");
+     ("addr_map", "(address,tez) map");
+     ("Coq.Init.Datatypes.nat", "nat")].
+
+(** A translation table for primitive binary operations *)
+Definition TT : env string :=
+  [("Coq.ZArith.BinInt.Z.add", "addTez");
+     ("PeanoNat.Nat.ltb", "ltbN");
+     ("PeanoNat.Nat.leb", "lebN");
+     ("PeanoNat.Nat.eqb", "eqN");
+     ("Coq.ZArith.BinInt.Z.leb", "lebTez");
+     ("Coq.ZArith.BinInt.Z.ltb", "ltbTez");
+     ("negb", "not");
+     ("add_map", "Map.add");
+     ("lookup", "Map.find")].
+
+Compute liquidifyModule TT TTty CFModule.
